README.md
@@ -10,6 +10,7 @@ assistant.
 
 Use the Nix flake-based ecosystem for working with this repository.
 `nix develop` enters a shell environment with the necessary dependencies
-available.
+available. It's also possible to automatically enter the development environment
+using a tool like `nix-direnv`.
 
-`isabelle jedit` launches the IDE.
+`isabelle jedit` launches the IDE from the command line.
